implicit bug again?

src/tls/IK.fst
@@ -1,5 +1,8 @@
 module IK 
 
+open FStar.HyperStack
+open FStar.HyperStack.ST
+
 /// a standalone experiment modelling key derivation parametrically in
 /// the use of the derived keys.
 ///
@@ -10,13 +13,14 @@ module IK
 ///
 /// Not done yet: conditional idealization and erasure.
 
-assume type lbytes (len:UInt32.t)
+type bytes = Platform.Bytes.bytes
+let lbytes (len:UInt32.t) = Platform.Bytes.lbytes (UInt32.v len)
 assume val sample: len:UInt32.t -> lbytes len  // not pure!
 
 /// How to deal with agility etc? Key (i:id) (u:usage) where u is
 /// concrete, and usually bound to i---in which case it is Ok to
 /// select u at derivation-time.
- 
+  
 /// --------------------------------------------------------------------------------------------------
 /// We embed first-class modules as datatype "packages"
 ///
@@ -32,12 +36,22 @@ noeq type ipkg = | Idx:
 /// Keyed functionality define Key packages, parametric in their
 /// indexes, but concrete on their key randomness; instances may have
 /// any number of other functions (such a leak, for instance).
+
+/// Derived key length restriction when using HKDF
+type keylen = l:UInt32.t {UInt32.v l <= 256} 
+
 noeq type pkg (ip:ipkg) = | Pkg:
   use: Type0 -> 
   key: (ip.t -> use -> Type0) -> 
-  len: (use -> UInt32.t) ->
-  create: (i:ip.t -> u:use -> key i u) -> 
-  coerce: (i:ip.t {~(ip.honest i)} -> u:use -> lbytes (len u) -> key i u) ->
+  len: (use -> keylen) ->
+  create: (
+    i:ip.t -> u:use -> ST (key i u)
+    (requires fun h0 -> True)
+    (ensures fun h0 p h1 -> True)) -> 
+  coerce: (
+    i:ip.t -> u:use -> lbytes (len u) -> ST (key i u)
+    (requires fun h0 -> ~(ip.honest i))
+    (ensures fun h0 p h1 -> True)) ->
   pkg ip
 
 /// pick an ordering: ip.t -> use for now.
@@ -52,6 +66,7 @@ noeq type pkg (ip:ipkg) = | Pkg:
 /// sample agile functionality,
 
 type aeadAlg = | AES_GCM128 | AES_GCM256
+val aeadLen: aeadAlg -> keylen 
 let aeadLen = function
   | AES_GCM128 -> 32ul
   | AES_GCM256 -> 48ul
@@ -72,7 +87,6 @@ let encrypt #ip #i #a k v = v + 1
 /// a default functionality (no idealization);
 /// for modelling, we could also provide a "leak" function
 ///
-type keylen = n:UInt32.t { UInt32.v n < 128 }
 type raw  (#ip: ipkg) (i: Idx?.t ip) (len:keylen) = lbytes len
 let create_raw (#ip: ipkg) (i: ip.t) (len:keylen): raw  i len = sample len
 let coerce_raw (#ip: ipkg) (i: ip.t) (len:keylen) (r:lbytes len): raw i len = r
@@ -82,20 +96,39 @@ let rp (ip:ipkg): pkg ip = Pkg keylen raw (fun n -> n) create_raw coerce_raw
 /// module Index
 
 /// We provide an instance of ipkg to track key derivation (here using constant labels)
-type label = string 
+type label = bytes
 
-/// We expect this function to be fully applied at compile time.
-type usage (a:Type0) (ip:ipkg) =  label -> p:pkg ip & (ctx:a -> p.use)
+/// We expect this function to be fully applied at compile time,
+/// returning a package and a algorithm-derivation function to its
+/// agility parameter (to be usually applied at run-time).
+/// 
+type usage (a:Type0) (ip:ipkg) =
+  label -> p:pkg ip & (ctx:a -> p.use)
 
-type id_dhe = nat // simplification: instead of the index, use  materials (g,X,Y)
+type id_dhe = g: CommonDH.group & gX: CommonDH.share g & CommonDH.share g
 type id_psk = nat // external application PSKs only; we may need a special PSK0 constructor too
 type id = 
   | Zero // symbolic constant for absent extraction arguments
   | Preshared of id_psk  // external application PSKs only
   | Extract0: materials:id -> id
-  | Extract1: salt:id -> materials: id_dhe -> id // do we need 2 cases?
+  | Extract1: salt:id -> materials: id_dhe -> id 
+// do we need 2 cases?
+//| ExtractWide1: salt:id -> #g: CommonDH.group -> CommonDH.share g -> id // do we need 2 cases?
   | Extract2: salt:id  -> id
   | Derived: id -> label -> id  
+
+// 17-10-17 Discussion with Markulf
+//
+// We'd rather keep wide indexes secret.  Internally, for each salt
+// index, we maintain a table from (g, gX, gY) to PRFs, with some
+// sharing.  (The sharing may be public, but not wide indexes values
+// are not.)  Informally this is sound because our limited use of the
+// tables does not depend on their sharing.
+//
+// The danger of overly precise indexes is that, ideally, we may
+// separate instances that use the same concrete keys---in our case
+// this does not matter because security does not depend on their
+// sharing.
 
 /// Using different constructors for different constructions; we don't
 /// restrict index, but we only provide the key-level operations at
@@ -124,19 +157,61 @@ let ii:ipkg = Idx id (fun _ -> true)
 /// we define a KDF parametric in both its usage and ipkg
 /// We rely on type abstraction to separate secrets with different indexes
 /// For soundness, we must also prevent external calls to create derived secrets.
-type kdfa = | SHA1 | SHA2
+///
+/// We idealize KDF as a random function, with lazy sampling.
+/// This holds syntactically only after inlining all calls to
+/// pkg.create/coerce.
+/// 
+/// This requires memoizing calls, which is a bit tricky when calling
+/// stateful allocators.
+/// 
+type kdfa = Hashing.Spec.alg
 type info = {ha:kdfa; aea:aeadAlg} (* runtime *) 
 //type suse = a:info * usage info ii
 
-let secret_len a = 
-  match a.ha with 
-  | SHA1 -> 8ul
-  | SHA2 -> 16ul 
-assume new type secret 
-  (ip: ipkg) 
-  (u: usage info ip)
-  (i: ip.t) 
+let derived_key (u: usage info ii) (i: ii.t) (v:label) (a: info) = 
+  let (| pkg', derived_alg |) = u v in 
+  pkg'.key (Derived i v) (derived_alg a)
+
+let there: FStar.Monotonic.RRef.rid = admit() 
+
+private type table 
+  // (ip: ipkg) 
+  (u: usage info ii)
+  (i: ii.t) 
   (a: info) 
+= MonotoneMap.t there label (fun v -> derived_key u i v a) (fun _ -> True)
+
+let secret_len a = UInt32.uint_to_t (Hashing.Spec.tagLen (a.ha))
+ 
+let lookup   
+  (#u: usage info ii)
+  (#i: ii.t) 
+  (#a: info) 
+  (t: table u i a) = MonotoneMap.lookup t 
+let extend 
+  (#u: usage info ii)
+  (#i: ii.t) 
+  (#a: info) 
+  (t: table u i a) = MonotoneMap.extend t 
+
+// when to be parametric on ip? not for the KDF itself: we use ip's constructors.
+let secret 
+  // (ip: ipkg) 
+  (u: usage info ii)
+  (i: ii.t) 
+  (a: info) : Type0
+=
+  if ii.honest i 
+  then table u i a
+  else lbytes (secret_len a)
+
+let ideal_secret 
+  (#u: usage info ii)
+  (#i: ii.t { ii.honest i})
+  (#a: info)
+  (t: table u i a): secret u i a = t 
+
 
 /// Real KDF schemes, parameterized by an algorithm computed from the
 /// index (existing code).
@@ -147,63 +222,73 @@ assume new type secret
 /// MK: what does reverse-inline of low-level KeyGen mean?
 
 val coerce: 
-  ip: ipkg ->
-  u: usage info ip ->
-  i: ip.t ->
+//ip: ipkg ->
+  u: usage info ii ->
+  i: ii.t ->
   a: info (* run-time *) -> 
   repr: lbytes (secret_len a) -> 
-  secret ip u i a 
-let coerce ip u i a repr = admit()
+  ST (secret u i a)
+  (requires fun h0 -> ~(ii.honest i))
+  (ensures fun h0 p h1 -> True)
+let coerce u i a repr = repr
 
 val create: 
-  ip: ipkg ->
-  u: usage info ip -> 
-  i: ip.t ->
+//ip: ipkg ->
+  u: usage info ii -> 
+  i: ii.t ->
   a: info (* run-time *) ->
-  secret ip u i a
-let create ip u i a = 
-  let raw = sample (secret_len a) in
-  coerce ip u i a raw
+  ST (secret u i a)
+  (requires fun h0 -> True)
+  (ensures fun h0 r h1 -> True)
+let create u i a = 
+  if ii.honest i 
+  then 
+    //style: how to avoid repeating those parameters?
+    MonotoneMap.alloc #there #label #(fun v -> derived_key u i v a) #(fun _ -> True) 
+  else 
+    coerce u i a (sample (secret_len a)) 
 
-let pp (ip:ipkg) (u: usage info ip): pkg ip = Pkg 
+let pp (* ip:ipkg *) (u: usage info ii): pkg ii = Pkg 
   info
-  (secret ip u) 
+  (secret u) 
   secret_len
-  (create ip u) 
-  (coerce ip u)
+  (create u) 
+  (coerce u)
 
 /// TODO consider separating pp packages more explicitly, so that we
 /// can idealize them one at a time. (Having one proof step for each
 /// nested level of key derivation seems unavoidable.)
 
-let derived_key (u: usage info ii) (i: id) (v:label) (a: info) = 
-  let (| pkg', derived_alg |) = u v in 
-  pkg'.key (Derived i v) (derived_alg a)
 
+inline_for_extraction
 val derive:
   #u: usage info ii ->
   #i: id ->
-  a: info -> 
-  k: secret ii u i a ->
+  #a: info -> 
+  k: secret u i a ->
   v: label ->
-  derived_key u i v a 
-
-let derive  #u #i a k v = 
-  let (| pkg', derived_alg |) = u v in 
+  ST (derived_key u i v a)
+  (requires fun h0 -> True)
+  (ensures fun h0 r h1 -> True)
+ 
+let derive  #u #i #a k v = 
+  let (| pkg, derived_alg |) = u v in 
   let a' = derived_alg a in 
-  if ii.honest (*safe*) i // (Derived i v) 
+  if ii.honest (*safe*) i 
   then
-    pkg'.create (Derived i v) a' //keybytes 
+    match MonotoneMap.lookup k v with 
+    | Some dk -> dk
+    | None -> 
+      let dk = pkg.create (Derived i v) a' in 
+      MonotoneMap.extend k v dk;
+      dk
   else 
-    let raw = sample (pkg'.len a') in 
-    pkg'.coerce (Derived i v) a' raw
+    let raw =
+      HKDF.expand #(a.ha) k v (UInt32.v (pkg.len a')) in 
+    pkg.coerce (Derived i v) a' raw
 
+(*
 /// Reconsider packaging: should create take external randomness?
-///
-/// core idealized functionality, presumably called at most once on every v. 
-/// full coercion is something different. 
-/// otherwise, create suffices for all purposes.
-
 
 /// --------------------------------------------------------------------------------------------------
 /// PSKs, Salt, and Extraction (can we be more parametric?)
@@ -286,41 +371,187 @@ assume val extract0:
   k: psk #ii #u i a -> 
   secret ii u (Extract0 i) a
 
+
 /// HKDF.Extract(key=s, materials=dh_secret) idealized as 2-bit
 /// (KEF-ODH, KEF-Salt game); we will need separate calls for clients
 /// and servers.
-assume val extract1:
+
+/// we write prf_ for the middle salt-keyed extraction, conditionally
+/// idealized as a PRF keyed by salt1 depending on b1.
+/// 
+/// its interface provides create, coerce, leak, and extract
+/// its internal table memoizes it with *wide* domain gZ 
+
+/// Allocates a 
+/// Returns a narrow-indexed key, 
+/// 
+/// its internal state must ensure sharing
+///
+val prf_extract1:
   #u: usage info ii -> 
   #i: id ->
   #a: info -> 
   s: salt ii u i a ->
-  materials: id_dhe -> 
-  secret ii u (Extract1 i materials) a
+  g: CommonDH.group ->
+  gX: CommonDH.share g -> 
+  gY: CommonDH.share g ->
+  gZ: CommonDH.share.g (* { dh gX gY gZ } *) ->
+  secret ii u (Extract1 i (| g, gX, gY |)) a
 
 (*
-assume type element
+let prf_extract1 #u #i #a s g gX gY gZ = 
+  let idh = (| g, gX, gY |) in
+  let j = Extract1 i idh in
+  let pkg = pp ii u in 
+  if ii.honest i & b1 
+  then 
+    if b2 then 
+    let 
+    let w = 
+      // "wide" PRF, memoized on gZ
+      match find s.wide gZ with 
+      | Some w -> w // may return k
+      | None -> 
+        let w = pkg.create0 j a in
+        s.wide := snoc s.wide w;
+        w in 
+    pkg.narrow j k 
+    // agreement on the algorithms follows from the salt.
+  else 
+    let raw = HKDF.extract (prf_leak s) gZ (* wide, concrete *) in 
+    pkg.coerce j a raw 
+*)
 
-/// Initiator computes DH keyshare
-assume val genDH:
-  g:element ->
-  iX:element
+val prf_leak:
+  #u: usage info ii -> 
+  #i: id ->
+  #a: info -> 
+  s: salt ii u i a -> bytes 
+// requires ~(honest i)
 
-/// Respoder computes DH secret material
-assume val extractR:
-  #expu: usage -> 
+
+(*
+/// ODH
+/// --------------------------------------------------------------------------------------------------
+
+assume val honest_gX: 
+  #g: CommonDH.group ->
+  gX: CommonDH.share g -> 
+  bool 
+
+// ideal state 
+// val peer: mref (map gX --> list (i,gY)) 
+// - presence codes I[X]
+// - contents codes R[X] 
+// conversely [keyshare] locally provides  x
+
+/// Client-side instance creation
+/// (possibly used by many honest servers)
+val odh_init:
+  g: CommonDH.group -> St (CommonDH.keyshare g)
+
+let odh_init g = 
+  let x = CommonDH.keygen g in 
+  let gX = CommonDH.pubshare y in  
+  // check gX is fresh;
+  // peer[gX] := []
+  x // also return gX?
+
+/// Server-side creation and completion
+///
+/// An elaboration of "derive" for two-secret extraction
+/// - kdf is the child KDF package.
+/// - HKDF is the concrete algorithm
+///
+val odh_test:
+  #u: usage info ii -> 
   #i: id -> 
-  s: salt expu ii i ->
-  iX: element ->
-  rY:element * id_dhe
+  #a: info -> 
+  s: salt ii u i a ->
+  g: CommonDH.group ->
+  gX: CommonDH.share g { honest_gX gX } -> 
+  ( gY:CommonDH.share g &
+  secret ii u (Extract1 i (| g, gX, gY |)) a )
+// requires peer[gX] defined.
+// I and R may not share the same salt (i)
+
+let odh_test #u #i #a s g gX = 
+  let y = CommonDH.keygen g in 
+  let gY = CommonDH.pubshare y in  
+  peer[gX] += (i, gY);
+  let idh = (| g, gX, gY |) in
+  let j = Extract1 i idh in 
+  let k = 
+    if b0 
+    then kdf.create j a (* narrow *)
+    else 
+      let gZ: commonDH.share g = admit() in 
+      let raw = HKDF.extract (prf_leak s) gZ (* wide, concrete *) in 
+      kdf.coerce j a raw 
+  in
+  gY, k (* TODO k is not registered yet *)
+
+// the PRF-ODH oracle, computing with secret exponent x
+val odh_prf:
+  #u: usage info ii -> 
+  #i: id -> 
+  #a: info -> 
+  s: salt ii u i a ->
+  g: CommonDH.group ->
+  x: CommonDH.keyshare g { honest_gX (CommonDH.pubshare x) } -> 
+  gY: CommonDH.share g -> 
+  secret ii u (Extract1 i (| g, CommonDH.pubshare x, gY |)) a 
+// requires peer[gX] is defined (witnessed in x) and does not contain (i,gY)
+// None? (find (i, gY) !peer[gX])
+
+let odh_prf #u #i #a s g x gY = 
+  let gX = CommonDH.pubshare x in
+  let gZ: CommonDH.share g = admit() in 
+  prf_extract1 s (| g, gX, gY |) gZ 
+
+/// --------------------------------------------------------------------------------------------------
+/// Diffie-Hellman shares
+/// module Extract1 
+
+// TODO: instead of CommonDH.keyshare g, we need an abstract stateful
+// [abstract type private_keyshare g = mref bool ...] that enables
+// calling it exactly once
+
+/// Initiator computes DH keyshare, irrespective of the KDF & salt. 
+let initI (g:CommonDH.group) = odh_init g 
+
+/// Responder computes DH secret material
+assume val extractR:
+  #u: usage info ii -> 
+  #i: id -> 
+  #a: info -> 
+  s: salt ii u i a ->
+  g: CommonDH.group ->
+  gX: CommonDH.share g ->
+  ( gY:CommonDH.share g &
+  secret ii u (Extract1 i (| g, gX, gY |)) a )
+
+let extractR #u #i #a s g gX = 
+  if honest_gX gX 
+  then ODH_test gX i
+  else
+    // real computation: gY is dishonest
+    let y = CommonDH.keygen g in 
+    let gY = CommonDH.pubshare y in  
+    let gZ: CommonDH.share g = admit() in // we could also use dh_responder
+    let k = extract1 s (| g, gX, gY |) gZ in
+    gY, k
 
 /// Initiator computes DH secret material
 assume val extractI: 
-  #expu: usage -> 
+  #u: usage info ii -> 
   #i: id -> 
-  s: salt expu ii i ->
-  iX: element ->
-  rY: element ->
-  id_dhe
+  #a: info ->
+  s: salt ii u i a ->
+  g: CommonDH.group ->
+  x: CommonDH.keyshare g ->
+  gY: CommonDH.share g ->
+  secret ii u (Extract1 i (| g, CommonDH.pubshare x, gY |)) a
 *)
 
 /// HKDF.Extract(key=s, materials=0) idealized as a single-use PRF.
@@ -340,14 +571,17 @@ assume val extract2:
 
 let some_keylen: keylen = 32ul
 
+inline_for_extraction
 let u_default:  p:pkg ii & (ctx:info -> p.use)  = (| rp ii, (fun (a:info) -> some_keylen) |)
 
+inline_for_extraction
 let u_traffic: usage info ii = function 
   | "ClientKey" | "ServerKey" -> (| mp ii , (fun (a:info) -> a.aea) |)
   | _ -> u_default
 
 // #set-options "--print_universes --print_implicits"
 
+inline_for_extraction
 let rec u_master_secret (n:nat ): Tot (usage info ii) (decreases (%[n; 0])) = function 
   | "traffic" -> (| pp ii u_traffic, (fun a -> a) |)
   | "resumption" -> if n > 0 then (| pskp ii (u_early_secret (n-1)), (fun (a:info) -> a)|) else (| rp ii, (fun (a:info) -> some_keylen) |)
@@ -387,7 +621,14 @@ let cipher  = encrypt k0 10
 val salt1:  salt ii (u_handshake_secret depth) (Derived i0 "salt") a
 let salt1  = derive a early_secret "salt"
 
-let i1 = Extract1 (Derived i0 "salt") 42
+let g = CommonDH.default_group
+let x = initI g 
+let gX = CommonDH.pubshare x
+let gY: CommonDH.share g = admit()
+let dhe_id: id_dhe = (| g, gX, gY |)
+
+let i1 = Extract1 (Derived i0 "salt") dhe_id
+
 
 (*
 assume val g:element
@@ -395,7 +636,8 @@ let iX = genDH g
 *)
 
 val hs_secret : secret ii (u_handshake_secret depth) i1 a
-let hs_secret = extract1 salt1 42 
+// let hs_secret = extract1 salt1 42 
+let hs_secret = extractI salt1 g x gY
 
 val hs_traffic: secret ii u_traffic (Derived i1 "traffic") a
 let hs_traffic = derive a hs_secret "traffic"
@@ -450,3 +692,4 @@ let next_early_secret = extract0 rsk
 //
 // let k1' = derive k0 "secret" 
 // let k2' = derive #(u 22)  k1'  "aead"  // the type is not normalized; the key is not usable.
+*)
